src/Protocol.v
@@ -9,6 +9,8 @@ Require Import CrossCrypto.FirstOrder.
 Require Import CrossCrypto.Tuple.
 Require Import CrossCrypto.HList.
 Require Import CrossCrypto.Tail.
+Require Import CrossCrypto.Execution.
+Require Import Omega.
 
 Definition head T (l : list T) (H : l <> []) : T.
   destruct l.
@@ -91,6 +93,8 @@ Section Protocols.
     mkProtocol {
         Q : nat -> Type;
         q0 : Q 0;
+        N_cap : nat;
+        fin_Q : forall n : nat, Q n -> n < N_cap;
         transition : forall n, Q n -> Q (S n) -> Type := @transition_ Q;
         transitions : forall n (q : Q n),
                         list {q' : Q (S n) & transition q q'};
@@ -103,93 +107,122 @@ Section Protocols.
                          message
       }.
 
-  Inductive execution (p : protocol)
-  : forall n, p.(Q) n -> tuple (term message) n ->
-              tuple (term message) (n + length p.(initial_knowledge))
-              -> Type :=
-  | Initial : execution p.(q0) t[] (list_to_tuple p.(initial_knowledge))
-  | Transition :
-      forall n (q : p.(Q) n) inputs knowledge q' (t : transition q q'),
-        execution q inputs knowledge ->
-        let new_input := (App (p.(handles) n)
-                              (tuple_to_hlist knowledge)) in
-        let new_inputs := new_input t:: inputs in
-        let new_knowledge :=
-            t.(output) inputs new_input t:: knowledge in
-        execution q' new_inputs new_knowledge.
+  Definition initial_knowledge_t p := list_to_tuple p.(initial_knowledge).
 
-  Definition valid_exec (m : model) (p : protocol)
-             n (q : p.(Q) n) inputs knowledge
-             (e : execution q inputs knowledge) : Prop.
-    induction e.
-    exact True.
-    set (guard_condition := (fun t_ : {q' : Q p (S n) & transition q q' } =>
-                              let t := projT2 t_ in
-                              m.(interp_term) (t.(guard) inputs new_input) =
-                              m.(interp_term) (App ftrue h[]))).
-    exact (exists t_ l,
-             In_with_tail t_ l (transitions q) /\
-             (eq_2 (projT2 t_) t) /\
-             guard_condition t_ /\
-             (forall t'_, In t'_ l -> ~guard_condition t'_)).
-  Defined.
+  Definition machine_state p :=
+    {n : nat & p.(Q) n * tuple (term message) n *
+               tuple (term message) (n + length p.(initial_knowledge))}%type.
+  Definition machine_initial p : machine_state p :=
+    existT _ 0 (q0 p, t[], initial_knowledge_t p).
 
-  Lemma valid_exec_extension_unique :
-    forall (m : model) (p : protocol) n (q : p.(Q) n) inputs knowledge
-           (e : execution q inputs knowledge)
-           q' (t : transition q q') q'1 (t1 : transition q q'1),
-      valid_exec m (Transition t e) -> valid_exec m (Transition t1 e) ->
-      (eq_2 t t1).
-    intros m p n q inputs knowledge e q' t q'1 t1 Hv Hv1.
-    simpl in Hv.
-    destruct Hv as [t_ [l [Iwt [[eq' et] [Hguard Hguardrest]]]]].
-    subst q'.
-    subst t.
-    simpl in Hv1.
-    destruct Hv1 as [t_1 [l1 [Iwt1 [[eq'1 et1] [Hguard1 Hguardrest1]]]]].
-    subst q'1.
-    subst t1.
-    simpl.
+  Inductive transition_valid (m : model) (p : protocol) n :
+    p.(Q) n -> tuple (term message) n ->
+    tuple (term message) (n + length p.(initial_knowledge)) ->
+    p.(Q) (S n) -> tuple (term message) (S n) ->
+    tuple (term message) (S n + length p.(initial_knowledge)) -> Prop :=
+  | TransValid q inputs knowledge t_ l :
+      let q' := projT1 t_ in
+      let t := projT2 t_ in
+      let new_input := (App (p.(handles) n)
+                            (tuple_to_hlist knowledge)) in
+      let new_inputs := new_input t:: inputs in
+      let new_knowledge :=
+          t.(output) inputs new_input t:: knowledge in
+      let guard_condition := (fun t_ : {q' : Q p (S n) & transition q q'} =>
+                                let t := projT2 t_ in
+                                m.(interp_term) (t.(guard) inputs new_input) =
+                                m.(interp_term) (App ftrue h[])) in
+      In_with_tail t_ l (transitions q) ->
+      guard_condition t_ ->
+      (forall t'_, In t'_ l -> ~guard_condition t'_) ->
+      transition_valid m q inputs knowledge q' new_inputs new_knowledge.
 
-    assert (t_ = t_1) as Heqt_.
+  Lemma valid_transition_unique (m : model) (p : protocol) n
+        (q : p.(Q) n) inputs knowledge
+        q'1 inputs'1 knowledge'1
+        q'2 inputs'2 knowledge'2 :
+    transition_valid m q inputs knowledge q'1 inputs'1 knowledge'1 ->
+    transition_valid m q inputs knowledge q'2 inputs'2 knowledge'2 ->
+    q'1 = q'2 /\ inputs'1 = inputs'2 /\ knowledge'1 = knowledge'2.
+    intros V1 V2.
+    inversion_clear V1 as [? ? knowledge1 t_1 l1 q'1_ t1 new_input1
+                             inputs'1_ knowledge'1_ guard1 ? HG1 HNG1].
+    inversion_clear V2 as [? ? knowledge2 t_2 l2 q'2_ t2 new_input2
+                             inputs'2_ knowledge'2_ guard2 ? HG2 HNG2].
+    subst.
+    replace guard2 with guard1 in * by reflexivity; clear guard2.
 
-    set (new_input := (App (p.(handles) n)
-                              (tuple_to_hlist knowledge))).
-    set (guard_condition := (fun t_ : {q' : Q p (S n) & transition q q' } =>
-                              let t := projT2 t_ in
-                              m.(interp_term) (t.(guard) inputs new_input) =
-                              m.(interp_term) (App ftrue h[]))).
-    eapply head_unique_prop with (P := guard_condition); eassumption.
-    subst t_1.
-    refine (eq_refl2 (H:=eq_refl) _).
-    reflexivity.
+    assert (t_1 = t_2) by
+        (eapply head_unique_prop with (P := guard1); eassumption).
+    subst t_2.
+    split; [|split]; reflexivity.
   Qed.
 
-  Inductive Execution (p : protocol) : Type :=
-  | exec : forall n (q : p.(Q) n) inputs knowledge
-                  (e : execution q inputs knowledge), Execution p.
+  Definition machine_lt (m : model) p (to from : machine_state p) : Prop.
+    destruct from as [n [[q i] k]].
+    destruct to as [n' [[q' i'] k']].
+    refine (exists H : n' = S n, _).
+    subst n'.
+    exact (transition_valid m q i k q' i' k').
+  Defined.
 
-  Definition valid_Exec (m : model) (p : protocol) (e : Execution p) : Prop :=
-    match e with
-      | exec e => valid_exec m e
-    end.
+  Definition nat_gt_max_wf (N : nat) (A : nat -> Type)
+          (cap : forall n, A n -> n < N)
+          (A_lt : sigT A -> sigT A -> Prop)
+          (A_lt_gt : forall a a' : sigT A, A_lt a' a -> projT1 a' > projT1 a) :
+    well_founded A_lt.
+    assert (forall n (a : A n), exists b, n = N - b) as HcN.
+    {
+      intros n a.
+      exists (N - n).
+      specialize (cap n a).
+      omega.
+    }
+    intros [n a].
+    destruct (HcN n a) as [b].
+    subst n.
+    refine ((Fix lt_wf (fun n => forall a : A (N - n),
+                                   Acc A_lt (existT _ _ a)) _) b a); clear a b.
+    intros b H a.
+    constructor.
+    intros a' l.
+    destruct a' as [n' a'].
+    destruct (HcN n' a') as [b'].
+    subst n'.
+    apply H.
+    specialize (A_lt_gt (existT _ _ a) (existT _ _ a') l).
+    simpl in A_lt_gt.
+    omega.
+  Defined.
 
-  Definition final_exec (p : protocol) (e : Execution p) : Prop :=
-    match e with
-      | @exec _ _ q _ _ _ => final q
-    end.
+  Definition machine_lt_wf (m : model) p : well_founded (@machine_lt m p).
+    eapply nat_gt_max_wf.
+    - intros n [[q _] _].
+      apply fin_Q; eassumption.
+    - intros [n [[q i] k]] [n' [[q' i'] k']] [H _].
+      simpl.
+      omega.
+  Defined.
 
-  Theorem exec_final_valid_unique :
-    forall (m : model) (p : protocol) (e e' : Execution p),
-      final_exec e -> final_exec e' -> valid_Exec m e -> valid_Exec m e' ->
-      e = e'.
-    intros m p e e'' Hfe Hfe'' Hve Hve''.
-    destruct e as [n q inputs knowledge e].
-    destruct e'' as [n' q' inputs' knowledge' e''].
-    generalize e'' Hfe'' Hve''.
-    induction e.
-    intros e' Hfe' Hve'.
-  Admitted.  (* TODO *)
+  Definition model_protocol_machine m p :=
+    @mkMachine (machine_state p) (machine_initial p)
+               (@machine_lt m p) (@machine_lt_wf m p).
+
+  Theorem machine_unique m p : unique_transition (model_protocol_machine m p).
+    intros x x'1 x'2 t1 t2.
+    simpl in t1, t2.
+    unfold machine_lt in t1, t2.
+    destruct x as [n [[q i] k]].
+    destruct x'1 as [n'1 [[q'1 i'1] k'1]].
+    destruct x'2 as [n'2 [[q'2 i'2] k'2]].
+    destruct t1 as [H1 tv1], t2 as [H2 tv2].
+    subst n'1.
+    subst n'2.
+    unfold eq_rect_r in tv1; simpl in tv1.
+    unfold eq_rect_r in tv2; simpl in tv2.
+    destruct (valid_transition_unique tv1 tv2) as [qe [ie ke]].
+    rewrite qe, ie, ke; reflexivity.
+  Qed.
 
   (* Existence of a final valid execution requires at least decidability
   over domain bool *)
